WIP SI trace proof

aneris/examples/transactional_consistency/snapshot_isolation/trace/implication_trace.v
@@ -14,19 +14,139 @@ From aneris.examples.transactional_consistency Require Import user_params aux_de
 Section trace_proof.
   Context `{!anerisG Mdl Σ, !User_params}.
 
+  (** Definitons and lemmas for the wrapped resources *)
+  
+  Definition rel_exec_map (exec : execution) (m : gmap Key (list val)) :=
+    ∃ s, last (split exec).2 = Some s ∧
+      (∀ k ov h, s !! k = ov ↔ (m !! k = Some h ∧ last h = ov)) ∧
+      (∀ k h v_i v_j i j, m !! k = Some h → h !! i = Some v_i → h !! j = Some v_j → i < j →
+        ∃ s_i' s_j' i' j', (split exec).2 !! i' = Some s_i' ∧ (split exec).2 !! j' = Some s_j' ∧ i' < j') ∧
+      (∀ k s_i s_j i j, (split exec).2 !! i = Some s_i → (split exec).2 !! j = Some s_j → i < j → 
+        ∃ h v_i' v_j' i' j', m !! k = Some h ∧ h !! i' = Some v_i' ∧ h !! j' = Some v_j' ∧ i' < j').
+
+  Definition reads_from_last_state (exec : execution) (k : Key) (v : val) := 
+    ∃ s, last (split exec).2 = Some s ∧ s !! k = Some v.
+
+  Definition GlobalInvExtSI (γ : gname) (T : list transaction) (exec : execution) : iProp Σ := 
+    ⌜∀ trans s k v, trans ∈ T → (Rd s k (Some v)) ∈ trans → 
+      (¬ ∃ s' v', rel_list trans (Wr s' k v') (Rd s k (Some v))) →
+        reads_from_last_state exec k v⌝.
+
+  Lemma valid_execution_rc_imp exec_pre m_pre exec m s st trans T :
+    rel_exec_map exec_pre m_pre →
+    rel_exec_map exec m →
+    exec_pre `prefix_of` exec →
+    (∀ s k v, Wr s k v ∈ trans → ∃ h, m_pre !! k = Some h ∧ m !! k = Some h) →
+    optional_applied_transaction exec st (trans ++ [Cm s true]) →
+    based_on exec T →
+    (trans ++ [Cm s true]) ∉ T →
+    (∀ s k v, Rd s k (Some v) ∈ trans → 
+      (¬ (∃ s' v', rel_list trans (Wr s' k v') (Rd s k (Some v)))) → 
+      reads_from_last_state exec_pre k v) →
+    valid_execution commit_test_si exec →
+    valid_execution commit_test_si (exec ++ [((trans ++ [Cm s true]), st)]).
+  Proof.
+    intros Hrel_ex Hrel_ex' Hpre Hwrites Happl Hbased Hnin Hreads Hvalid.
+    split_and!.
+    - destruct Happl as [(s' & t' & Hlast & Happl)|Hfalse].
+      + intros i eq e2. 
+        eapply extend_execution_imp; try done.
+      + rewrite /valid_execution in Hvalid.
+        rewrite last_None in Hfalse.
+        set_solver.
+    - destruct Hvalid as (_ & Hvalid & _).
+      rewrite lookup_app_Some.
+      set_solver.
+    - intros t Hin.
+      rewrite split_split in Hin.
+      simpl in Hin.
+      rewrite elem_of_app in Hin.
+      pose proof Hvalid as Hvalid'.
+      destruct Hvalid as (_ & _ & Hvalid & _).
+      destruct Hin as [Hin|Hin].
+      + destruct (Hvalid t Hin) as (s' & Hin_s' & Hcompl & Hno_conf).
+        exists s'.
+        split_and!.
+        * rewrite split_split.
+          simpl. 
+          set_solver.
+        * intros tag c k ov i Hlookup_i Hrd_in.
+          assert (read_state c k ov i exec s') as (j & Hleq & Hlookup_j & Hlookup_k).
+          {
+            apply (Hcompl tag c k ov i); last done.
+            rewrite split_split in Hlookup_i.
+            simpl in Hlookup_i.
+            rewrite lookup_app_Some in Hlookup_i.
+            destruct Hlookup_i as [Hlookup_i|Hlookup_i]; first done.
+            exfalso.
+            apply Hnin.
+            rewrite list_lookup_singleton_Some in Hlookup_i.
+            destruct Hlookup_i as (_ & _ & Hlookup_i).
+            rewrite Hlookup_i.
+            apply (Hbased t).
+            split; first done.
+            rewrite -Hlookup_i; intros Hfalse. 
+            destruct trans; set_solver.
+          }
+          exists j.
+          split_and!; try done.
+          rewrite split_split.
+          simpl.
+          rewrite lookup_app_Some.
+          by left.
+        * intros i j Hlookup_i Hlookup_j i' t' Hlt Hlookup_i'.
+          eapply (Hno_conf i j _ _ i'); try done.
+          rewrite split_split in Hlookup_i'.
+          simpl in Hlookup_i'.
+          rewrite lookup_app_Some in Hlookup_i'.
+          destruct Hlookup_i' as [Hlookup_i'|Hlookup_i']; first done.
+          exfalso.
+          rewrite split_split in Hlookup_j.
+          simpl in Hlookup_j.
+          rewrite lookup_app_Some in Hlookup_j.
+          destruct Hlookup_j as [Hlookup_j|(_ & Hlookup_j)].
+          -- apply lookup_lt_Some in Hlookup_j.
+             lia.
+          -- rewrite list_lookup_singleton_Some Nat.sub_0_le in Hlookup_j.
+             lia.
+      + assert (t = trans ++ [Cm s true]) as ->; first set_solver.
+        destruct Hrel_ex as (s_snap & Hrel_ex).
+        exists s_snap.
+        split_and!.
+        * admit.
+        * admit.
+        * admit.
+    - intros t1 t2 i j Hlookup_i Hlookup_j Heq.
+      rewrite split_split in Hlookup_i; simpl in Hlookup_i.
+      rewrite split_split in Hlookup_j; simpl in Hlookup_j.
+      rewrite lookup_snoc_Some in Hlookup_i.
+      rewrite lookup_snoc_Some in Hlookup_j.
+      destruct Hvalid as (_ & _ &  _ & Hvalid).
+      destruct Hlookup_i as [Hlookup_i|(Hlength_i & Heq_i)]; 
+        destruct Hlookup_j as [Hlookup_j|Hlookup_j].
+      1, 4 : set_solver.
+      all : subst.
+      all : exfalso.
+      all : apply Hnin.
+      all : apply Hbased.
+      all : split; first (apply elem_of_list_lookup; set_solver).
+      all : intros Hfalse; destruct trans; set_solver.
+  Admitted.
+
   (** Wrapped resources  *)
-  Global Program Instance wrapped_resources `(res : !SI_resources Mdl Σ) : SI_resources Mdl Σ :=
+  Global Program Instance wrapped_resources (γmstate : gname) (clients : gset socket_address)
+  `(res : !SI_resources Mdl Σ) : SI_resources Mdl Σ :=
     {|
       GlobalInv := True%I;
       OwnMemKey k V := True%I;
       OwnLocalKey k c vo := True%I;
-      ConnectionState c s sa := True%I;
+      ConnectionState c sa s := (ConnectionState c sa s ∗ ghost_map_elem γmstate sa (DfracOwn 1%Qp) (s, Some c))%I;
       IsConnected c sa := True%I;
       KVS_si := KVS_si;
-      KVS_Init := True%I;
-      KVS_ClientCanConnect sa := True%I;
+      KVS_Init := KVS_Init%I;
+      KVS_ClientCanConnect sa := (KVS_ClientCanConnect sa ∗ ghost_map_elem γmstate sa (DfracOwn 1%Qp) (CanStart, None) ∗ ⌜sa ∈ clients⌝)%I;
       KeyUpdStatus v k b := True%I;
-      Seen k V := True%I;
+      Seen k V := Seen k V%I;
       extract c := res.(snapshot_isolation.specs.resources.extract) c;
     |}.
   Next Obligation.
